lib/generic_bv_ops.dfy
@@ -184,6 +184,37 @@ abstract module generic_bv_ops
         x / HW_BASE()
     }
 
+    function half_combine(lo: nat, hi: nat): (x: uint)
+        requires lo < HW_BASE();
+        requires hi < HW_BASE();
+        ensures x == lo + hi * HW_BASE();
+        ensures lh(x) == lo;
+        ensures uh(x) == hi;
+    {
+        Mul.LemmaMulNonnegative(hi, HW_BASE());
+        var temp:int := lo + hi * HW_BASE();
+        calc {
+            temp;
+            <
+            HW_BASE() + hi * HW_BASE();
+            {
+                Mul.LemmaMulProperties();
+            }
+            (hi + 1) * HW_BASE();
+            <=
+            {
+                Mul.LemmaMulInequality(hi + 1, HW_BASE(), HW_BASE());
+            }
+            HW_BASE() * HW_BASE();
+            BASE();
+        }
+        DivMod.LemmaFundamentalDivModConverse(temp, HW_BASE(), hi, lo);
+        Mul.LemmaMulIsCommutativeAuto();
+        reveal lh();
+        reveal uh();
+        temp
+    }
+
     lemma half_split_lemma(x: uint)
         ensures x == lh(x) + uh(x) * HW_BASE();
     {
